src/3d/Deps.fst
@@ -154,6 +154,7 @@ let scan_deps (fn:string) : ML scan_deps_t =
     | Probe_action_seq hd tl -> (deps_of_probe_action hd)@(deps_of_probe_action tl)
     | Probe_action_let i a k -> (deps_of_probe_atomic_action a)@(deps_of_probe_action k)
     | Probe_action_ite e th el -> deps_of_expr e @ deps_of_probe_action th @ deps_of_probe_action el
+    | Probe_action_array len b -> deps_of_expr len @ deps_of_probe_action b
   in
   let deps_of_params params : ML (list string) =
     params |> List.collect (fun (t, _, _) -> deps_of_typ t) in
